VLSM/SubProjectionTraces.v
@@ -1,0 +1,956 @@
+Require Import List Nat Bool.
+Import ListNotations.
+Require Import Lia.
+Require Import Logic.FunctionalExtensionality.
+
+Require Import Coq.Logic.FinFun Coq.Logic.Eqdep.
+
+From CasperCBC
+Require Import Lib.ListExtras Lib.Preamble VLSM.Common VLSM.Composition.
+
+Section SubProjectionTraces.
+
+Print sub_IM.
+
+Context
+  {message : Type}
+  {index : Type}
+  {IndEqDec : EqDecision index}
+  (IM : index -> VLSM message)
+  (sub_index_list : list index)
+  (Hi0_sub : sub_index_list <> [])
+  (sub_index : Type := sub_index sub_index_list)
+  (sub_index_eq_dec := sub_index_eq_dec sub_index_list)
+  (sub_index_prop := sub_index_prop sub_index_list)
+  (sub_index_prop_dec := sub_index_prop_dec sub_index_list)
+  (sub_IM : sub_index -> VLSM message := sub_IM IM sub_index_list)
+  .
+
+Existing Instance sub_index_prop_dec.
+
+Definition composite_state_sub_projection
+  (s : composite_state IM)
+  (subi : sub_index)
+  : vstate (sub_IM subi)
+  := s (proj1_sig subi).
+
+Definition composite_transition_item_sub_projection
+  (item : composite_transition_item IM)
+  (i := projT1 (l item))
+  (e : sub_index_prop i)
+  (j : sub_index := dec_exist _ i e)
+  : composite_transition_item sub_IM
+  :=
+  @Build_transition_item _ (composite_type sub_IM) (existT _ j (projT2 (l item))) (input item) (composite_state_sub_projection (destination item)) (output item).
+
+Definition composite_transition_item_sub_projection_proof_irrelevance
+  (item : composite_transition_item IM)
+  (i := projT1 (l item))
+  (e1 e2 : sub_index_prop i)
+  : composite_transition_item_sub_projection item e1 = composite_transition_item_sub_projection item e2.
+Proof.
+  destruct item. destruct l. unfold i in *. clear i.
+  unfold composite_transition_item_sub_projection.
+  simpl in *. f_equal.
+  match goal with
+  |- existT _ ?x1 _ = existT _ ?x2 _ => assert (Heq : x1 = x2)
+  end.
+  { apply dec_sig_eq_iff. reflexivity. }
+  simpl in *.
+  rewrite Heq.
+  assert (Heq : dec_exist sub_index_prop x e1 = dec_exist sub_index_prop x e2)
+  ; [|rewrite Heq].
+  unfold dec_exist. rewrite decide_True.
+  assert (dec_exist sub_index_prop x e1)
+
+
+Definition from_sub_projection
+  (a : composite_transition_item IM)
+  : Prop
+  := sub_index_prop (projT1 (l a)).
+
+Fixpoint finite_trace_sub_projection
+  (trx : list (composite_transition_item IM))
+  : list (composite_transition_item sub_IM)
+  :=
+  match trx with
+  | [] => []
+  | item :: trx =>
+    let tail := finite_trace_sub_projection trx in
+    match decide (from_sub_projection item) with
+    | left e => composite_transition_item_sub_projection item e :: tail
+    | _ => tail
+    end
+  end.
+
+Definition finite_trace_sub_projection_alt
+  (trx : list (composite_transition_item IM))
+  (ftrx := (filter (fun a => bool_decide (from_sub_projection a)) trx))
+  (Hall: Forall from_sub_projection ftrx := filter_Forall trx)
+  :=
+  List.map
+    (fun item : {a : composite_transition_item IM | from_sub_projection a} =>
+      let (item, e) := item in
+      composite_transition_item_sub_projection item e
+    )
+  (list_annotate from_sub_projection ftrx Hall).
+
+Lemma finite_trace_sub_projection_alt_cons
+  (item : composite_transition_item IM)
+  (trx : list (composite_transition_item IM))
+  : finite_trace_sub_projection_alt (item :: trx) =
+    let tail := finite_trace_sub_projection_alt trx in
+    match decide (from_sub_projection item) with
+    | left e => composite_transition_item_sub_projection item e :: tail
+    | _ => tail
+    end.
+Proof.
+  unfold finite_trace_sub_projection_alt at 1.
+  match goal with 
+  |- context [list_annotate _ _ ?all] =>
+    remember all as Hall
+  end.
+  clear HeqHall.
+  match goal with 
+  |- context [list_annotate _ ?f _] =>
+    remember f as flt
+  end.
+  simpl in Heqflt.
+  unfold bool_decide in Heqflt at 1.
+  unfold decide.
+  destruct (sub_index_prop_dec (projT1 (l item))) eqn:Hitem.
+  - subst flt.
+    rewrite list_annotate_unroll.
+    rewrite map_cons.
+  ; [|subst; reflexivity].
+  destruct (dec)
+  change (item :: trx) with ([item] ++ trx).
+  rewrite (filter_app _ [item] trx).
+  unfold filter.
+
+Lemma finite_trace_projection_list_alt_iff
+  (trx : list (composite_transition_item IM))
+  : finite_trace_sub_projection_alt trx = finite_trace_sub_projection trx.
+Proof.
+  induction trx; intros; [reflexivity|].
+  simpl.
+  destruct
+    (decide (from_sub_projection a)) eqn:Heq.
+      j =
+    (@projT1 index (fun n : index => @vlabel message (IM n))
+       (@l message (@composite_type message index IM) a))))
+    eqn:Heq.
+  - assert
+    (Hunroll :
+      filter (fun a => bool_decide (from_projection a)) (a :: trx)
+      = a :: filter (fun a => bool_decide (from_projection a)) trx
+    ).
+    { simpl.
+      unfold bool_decide, dec_from_projection, from_projection.
+      replace
+        (decide (j =
+        (@projT1 index (fun n : index => @vlabel message (IM n))
+           (@l message (@type message X) a))))
+      with
+        (@left
+           (@eq index j
+              (@projT1 index (fun n : index => @vlabel message (IM n))
+                 (@l message (@composite_type message index IM) a)))
+           (not
+              (@eq index j
+                 (@projT1 index (fun n : index => @vlabel message (IM n))
+                    (@l message (@composite_type message index IM) a)))) e)
+      .
+      reflexivity.
+    }
+    unfold finite_trace_projection_list_alt.
+    generalize dependent Hall.
+    rewrite Hunroll.
+    intro Hall.
+    rewrite list_annotate_unroll.
+    specialize (IHtrx (Forall_tl Hall)).
+    rewrite <- IHtrx.
+    simpl.
+    f_equal.
+    f_equal; try reflexivity.
+    replace (Forall_hd Hall) with e; try reflexivity.
+    apply UIP.
+  - assert
+    (Hunroll :
+      filter (fun a => bool_decide (from_projection a)) (a :: trx)
+      = filter (fun a => bool_decide (from_projection a)) trx
+    ).
+    { simpl.
+      unfold bool_decide, dec_from_projection, from_projection.
+      replace
+        (decide (j =
+        (@projT1 index (fun n0 : index => @vlabel message (IM n0))
+           (@l message (@type message X) a))))
+      with
+        (@right
+          (@eq index j
+             (@projT1 index (fun n : index => @vlabel message (IM n))
+                (@l message (@composite_type message index IM) a)))
+          (not
+             (@eq index j
+                (@projT1 index (fun n : index => @vlabel message (IM n))
+                   (@l message (@composite_type message index IM) a)))) n)
+        .
+      reflexivity.
+    }
+    unfold finite_trace_projection_list_alt.
+    generalize dependent Hall.
+    rewrite Hunroll.
+    intro Hall.
+    specialize (IHtrx Hall).
+    rewrite <- IHtrx.
+    reflexivity.
+Qed.
+
+Lemma finite_trace_projection_empty
+  (s : vstate X)
+  (trx : list (vtransition_item X))
+  (Htr : finite_protocol_trace_from X s trx)
+  (Hempty : finite_trace_projection_list trx = [])
+  (t : (vtransition_item X))
+  (Hin : In t trx)
+  : destination t j = s j.
+Proof.
+  generalize dependent t.
+  induction Htr; simpl; intros t Hin.
+  - inversion Hin.
+  - destruct l as [i l].
+    destruct H as [[[_om Hs'] [[_s Hiom] Hvalid]] Htransition].
+    unfold transition in Htransition; simpl in Htransition.
+    destruct (vtransition (IM i) l (s' i, iom)) as [si' om'] eqn:Hteq.
+    inversion Htransition; subst. clear Htransition.
+    destruct Hin as [Heq | Hin]; subst; simpl in *; destruct (decide (j = i)).
+    + inversion Hempty.
+    + apply state_update_neq. assumption.
+    + inversion Hempty.
+    + specialize (IHHtr Hempty t Hin). rewrite IHHtr.
+      apply state_update_neq. assumption.
+Qed.
+
+Lemma finite_trace_projection_list_app
+  (tr1 tr2 : list (composite_transition_item IM))
+  : finite_trace_projection_list (tr1 ++ tr2) =
+    finite_trace_projection_list tr1 ++ finite_trace_projection_list tr2.
+Proof.
+  induction tr1;[reflexivity|].
+  simpl.
+  match goal with
+  |- context [decide ?d] => destruct (decide d)
+  end
+  ; [|assumption].
+  simpl. rewrite IHtr1. reflexivity.
+Qed.
+
+Lemma preloaded_finite_trace_projection_last_state
+  (start : vstate X)
+  (transitions : list (vtransition_item X))
+  (Htr : finite_protocol_trace_from (pre_loaded_with_all_messages_vlsm X) start transitions)
+  (lstx := last (List.map destination transitions) start)
+  (lstj := last (List.map destination (finite_trace_projection_list transitions)) (start j))
+  : lstj = lstx j.
+Proof.
+  unfold lstx. unfold lstj. clear lstx. clear lstj.
+  induction Htr; try reflexivity.
+  destruct l as [i l].
+  rewrite map_cons.
+  rewrite unroll_last. simpl.
+  destruct (decide (j = i)).
+  - rewrite map_cons. rewrite unroll_last.
+    assumption.
+  - destruct H as [[[_om Hs'] [[_s Hiom] Hvalid]] Htransition].
+    unfold transition in Htransition; simpl in Htransition.
+    unfold vtransition in Htransition. simpl in Htransition.
+    destruct (vtransition (IM i) l (s' i, iom)) as [si' om'] eqn:Hteq.
+    inversion Htransition; subst. clear Htransition.
+    specialize (state_update_neq _ s' i si' j n); intro Hupd.
+    rewrite Hupd in *.
+    assumption.
+Qed.
+
+Lemma finite_trace_projection_last_state
+  (start : vstate X)
+  (transitions : list (vtransition_item X))
+  (Htr : finite_protocol_trace_from X start transitions)
+  (lstx := last (List.map destination transitions) start)
+  (lstj := last (List.map destination (finite_trace_projection_list transitions)) (start j))
+  : lstj = lstx j.
+Proof.
+  apply preloaded_finite_trace_projection_last_state.
+  apply VLSM_incl_finite_trace; [|assumption].
+  apply vlsm_incl_pre_loaded_with_all_messages_vlsm.
+Qed.
+
+Local Lemma _finite_ptrace_projection
+  (s : vstate X)
+  (Psj : protocol_state_prop Xj (s j))
+  (trx : list (vtransition_item X))
+  (Htr : finite_protocol_trace_from X s trx)
+   : finite_protocol_trace_from Xj (s j) (finite_trace_projection_list trx).
+Proof.
+  induction Htr.
+  - constructor. assumption.
+  - destruct l as [x lx]; simpl.
+    destruct H as [[Ps' [Piom [Hv Hc]]] Ht].
+    assert (Hpp : protocol_prop X (s, oom)).
+    { rewrite <- Ht. destruct Ps' as [_om Ps']. destruct Piom as [_s Piom].
+      apply protocol_generated with _om _s; try assumption. split; assumption.
+    }
+    assert (Hps : protocol_state_prop X s) by (exists oom; assumption).
+    destruct (decide (j = x)).
+    + subst x.
+      simpl in Ht.
+      destruct (vtransition (IM j) lx (s' j, iom)) as [si' om'] eqn:Hteq.
+      inversion Ht; subst. unfold composite_transition_item_projection_from_eq.
+      simpl.
+      rewrite state_update_eq in *.
+      simpl in Hv.
+      apply (finite_ptrace_extend Xj).
+      * apply IHHtr.
+        exists oom.
+        replace (@pair (@state message (@type message Xj)) (option message) si' oom)
+          with (vtransition (IM j) lx (s' j, iom)).
+        destruct Psj as [os'j Psj].
+        specialize (protocol_message_projection IM constraint j _ Piom); intros [sj HPjiom].
+        apply (protocol_generated Xj lx (s' j) os'j Psj sj iom HPjiom).
+        unfold valid; simpl.
+        exists s'.
+        split; try reflexivity.
+        split; try assumption.
+        split; try assumption.
+        destruct iom as [im|]
+        ; repeat split; assumption.
+      * assert
+          (Heqlx :
+            (@eq_rect_r index j (fun n : index => vlabel (IM n)) lx j (@eq_refl index j))
+            = lx
+          ) by reflexivity.
+        rewrite Heqlx.
+        specialize (protocol_message_projection IM constraint j _ Piom); intros HPjiom.
+        repeat split; try assumption.
+        exists s'.
+        repeat split; assumption.
+    + simpl in Ht. destruct (vtransition (IM x) lx (s' x, iom)) eqn:Hteq.
+      inversion Ht; subst.
+      rewrite state_update_neq in IHHtr; try assumption.
+      apply IHHtr.
+      assumption.
+Qed.
+
+Lemma protocol_state_projection
+  (s : state)
+  (Hps : protocol_state_prop X s)
+  : protocol_state_prop Xj (s j).
+Proof.
+  apply protocol_state_has_trace in Hps.
+  destruct Hps as [is [tr [[Htr His] Hs]]].
+  specialize (finite_trace_projection_last_state _ _ Htr) as Hlst.
+  apply _finite_ptrace_projection in Htr as Hptr.
+  - apply finite_ptrace_last_pstate in Hptr.
+    simpl in *.
+    rewrite Hlst in Hptr.
+    subst. assumption.
+  - apply initial_is_protocol. specialize (His j). assumption.
+Qed.
+
+(* The projection of a finite protocol trace remains a protocol trace *)
+
+Lemma finite_ptrace_projection
+  (s : vstate X)
+  (trx : list (vtransition_item X))
+  (Htr : finite_protocol_trace_from X s trx)
+   : finite_protocol_trace_from Xj (s j) (finite_trace_projection_list trx).
+Proof.
+  apply _finite_ptrace_projection; [|assumption].
+  apply protocol_state_projection.
+  apply finite_ptrace_first_pstate in Htr.
+  assumption.
+Qed.
+
+(* The projection of a preloaded finite protocol trace remains a preloaded protocol trace *)
+
+Lemma _preloaded_finite_ptrace_projection
+  (s : vstate X)
+  (Psj : protocol_state_prop (pre_loaded_with_all_messages_vlsm (IM j)) (s j))
+  (trx : list (vtransition_item X))
+  (Htr : finite_protocol_trace_from (pre_loaded_with_all_messages_vlsm X) s trx)
+   : finite_protocol_trace_from (pre_loaded_with_all_messages_vlsm (IM j)) (s j) (finite_trace_projection_list trx).
+Proof.
+  induction Htr.
+  - constructor. assumption.
+  - destruct l as [x lx]; simpl.
+    destruct H as [[Ps' [Piom [Hv Hc]]] Ht].
+    assert (Hpp : protocol_prop (pre_loaded_with_all_messages_vlsm X) (s, oom)).
+    { rewrite <- Ht. destruct Ps' as [_om Ps']. destruct Piom as [_s Piom].
+      apply protocol_generated with _om _s; try assumption. split; assumption.
+    }
+    assert (Hps : protocol_state_prop (pre_loaded_with_all_messages_vlsm X) s) by (exists oom; assumption).
+    destruct (decide (j = x)).
+    + subst x.
+      unfold vtransition in Ht. simpl in Ht.
+      unfold vtransition in Ht. simpl in Ht.
+      destruct (vtransition (IM j) lx (s' j, iom)) as [si' om'] eqn:Hteq.
+      inversion Ht; subst. 
+      unfold composite_transition_item_projection_from_eq. simpl.
+      rewrite state_update_eq in *.
+      simpl in Hv.
+      apply (finite_ptrace_extend (pre_loaded_with_all_messages_vlsm (IM j))).
+      * apply IHHtr.
+        exists oom.
+
+        replace
+          (@pair
+            (@state message
+              (@type message (@pre_loaded_with_all_messages_vlsm message (IM j))))
+            (option message)
+            si' oom)
+          with (vtransition (IM j) lx (s' j, iom)).
+        destruct Psj as [os'j Psj].
+        specialize (protocol_generated (pre_loaded_with_all_messages_vlsm (IM j)) lx (s' j) os'j Psj)
+          as Hgen.
+        specialize (Hgen (proj1_sig (vs0 (IM j))) iom).
+        spec Hgen; [apply (pre_loaded_with_all_messages_message_protocol_prop (IM j))|].
+        spec Hgen; [| apply Hgen].
+        assumption.
+      * assert
+          (Heqlx :
+            (@eq_rect_r index j (fun n : index => vlabel (IM n)) lx j (@eq_refl index j))
+            = lx
+          ) by reflexivity.
+        rewrite Heqlx.
+        split; [|assumption].
+        split; [assumption|].
+        split; [|assumption].
+        exists (proj1_sig (vs0 (IM j))).
+        apply (pre_loaded_with_all_messages_message_protocol_prop (IM j)).
+    + simpl in Ht. unfold vtransition in Ht.
+      simpl in Ht.
+      destruct (vtransition (IM x) lx (s' x, iom)) eqn:Hteq.
+      inversion Ht; subst.
+      rewrite state_update_neq in IHHtr by assumption.
+      apply IHHtr.
+      assumption.
+Qed.
+
+Lemma preloaded_protocol_state_projection
+  (s : state)
+  (Hps : protocol_state_prop (pre_loaded_with_all_messages_vlsm X) s)
+  : protocol_state_prop (pre_loaded_with_all_messages_vlsm (IM j)) (s j).
+Proof.
+  apply protocol_state_has_trace in Hps.
+  destruct Hps as [is [tr [[Htr His] Hs]]].
+  specialize (preloaded_finite_trace_projection_last_state _ _ Htr) as Hlst.
+  apply _preloaded_finite_ptrace_projection in Htr as Hptr.
+  - apply finite_ptrace_last_pstate in Hptr.
+    simpl in *.
+    rewrite Hlst in Hptr.
+    subst. assumption.
+  - apply initial_is_protocol. specialize (His j). assumption.
+Qed.
+
+Lemma preloaded_finite_ptrace_projection
+  (s : vstate X)
+  (trx : list (vtransition_item X))
+  (Htr : finite_protocol_trace_from (pre_loaded_with_all_messages_vlsm X) s trx)
+   : finite_protocol_trace_from (pre_loaded_with_all_messages_vlsm (IM j)) (s j) (finite_trace_projection_list trx).
+Proof.
+  apply _preloaded_finite_ptrace_projection; [|assumption].
+  apply preloaded_protocol_state_projection.
+  apply finite_ptrace_first_pstate in Htr.
+  assumption.
+Qed.  
+
+Lemma in_futures_projection
+  (s1 s2 : state)
+  (Hfutures : in_futures X s1 s2)
+  : in_futures Xj (s1 j) (s2 j).
+Proof.
+  destruct Hfutures as [tr [Htr Hs2]].
+  specialize (finite_ptrace_projection s1 tr Htr); intros Htrj.
+  exists (finite_trace_projection_list tr).
+  split; [assumption|].
+  subst s2.
+  apply finite_trace_projection_last_state.
+  assumption.
+Qed.
+
+Definition in_projection
+   (tr : Stream (composite_transition_item IM))
+   (n : nat)
+   := from_projection (Str_nth n tr).
+
+Definition in_projection_dec
+  := forall (tr : Stream (composite_transition_item IM)),
+       bounding (in_projection tr)
+       + { ss : monotone_nat_stream
+         | filtering_subsequence from_projection tr ss
+         }.
+
+Definition infinite_trace_projection_stream
+  (ss: Stream (composite_transition_item IM))
+  (ks: monotone_nat_stream)
+  (Hfilter: filtering_subsequence from_projection ss ks)
+  : Stream (vtransition_item (IM j))
+  :=
+  let subs := stream_subsequence ss ks in
+  let HForAll := stream_filter_Forall from_projection ss ks Hfilter in
+  let subsP := stream_annotate from_projection subs HForAll in
+  Streams.map
+    (fun item : {a : vtransition_item X | from_projection a} =>
+      let (item, e) := item in
+      let lj := eq_rect_r _ (projT2 (l item)) e in
+      @Build_transition_item _ (type Xj) lj (input item) (destination item j) (output item)
+    )
+    subsP.
+
+Lemma finite_trace_projection_stream
+  (ss: Stream (composite_transition_item IM))
+  (ks: monotone_nat_stream)
+  (Hfilter: filtering_subsequence from_projection ss ks)
+  (n : nat)
+  (kn := Str_nth n (proj1_sig ks))
+  (ss_to_kn := stream_prefix ss (succ kn))
+  (sproj := infinite_trace_projection_stream ss ks Hfilter)
+  : stream_prefix sproj (succ n) = finite_trace_projection_list ss_to_kn.
+Proof.
+  unfold sproj. unfold infinite_trace_projection_stream.
+  rewrite <- stream_prefix_map.
+  specialize
+    (stream_prefix_annotate
+      from_projection
+      (stream_subsequence ss ks)
+      (stream_filter_Forall from_projection ss ks Hfilter)
+      (succ n)
+    ); intros [Hall Heq].
+  clear -Heq.
+  match goal with
+  |- List.map _ ?s = _ => replace s with
+      (list_annotate from_projection (stream_prefix (stream_subsequence ss ks) (succ n)) Hall)
+  end.
+  specialize
+    (stream_filter_prefix
+       ss
+       ks
+       Hfilter
+       n
+    ); intros Hsfilter.
+  remember stream_prefix as sp.
+  simpl in Hsfilter. subst.
+  unfold succ in *.
+  generalize dependent Hall.
+  rewrite Hsfilter.
+  intros.
+  unfold ss_to_kn. unfold kn.
+  apply finite_trace_projection_list_alt_iff.
+Qed.
+
+Definition trace_projection
+  (Hproj_dec : in_projection_dec)
+  (tr : vTrace X)
+  : vTrace (IM j).
+Proof.
+  destruct tr as [s ls | s ss].
+  - exact (Finite (s j) (finite_trace_projection_list ls)).
+  - specialize (Hproj_dec ss).
+    destruct Hproj_dec as [[n1 _] | [ks Hfilter]].
+    + exact (Finite (s j) (finite_trace_projection_list (stream_prefix ss n1))).
+    + exact (Infinite (s j) (infinite_trace_projection_stream ss ks Hfilter)).
+Defined.
+
+Lemma trace_projection_initial_state
+  (Hproj_dec : in_projection_dec)
+  (tr : vTrace X)
+  : trace_first (trace_projection Hproj_dec tr)
+  = trace_first tr j.
+Proof.
+  destruct tr; try reflexivity.
+  simpl.
+  destruct (Hproj_dec s0).
+  - destruct b; reflexivity.
+  - destruct s1; reflexivity.
+Qed.
+
+Lemma infinite_ptrace_projection
+  (s: vstate X)
+  (ss: Stream transition_item)
+  (Psj: protocol_state_prop Xj (s j))
+  (Htr: infinite_protocol_trace_from X s ss)
+  (fs : monotone_nat_stream)
+  (Hfs: filtering_subsequence from_projection ss fs)
+  : infinite_protocol_trace_from Xj (s j) (infinite_trace_projection_stream ss fs Hfs).
+Proof.
+  apply infinite_protocol_trace_from_prefix_rev.
+  specialize (infinite_protocol_trace_from_prefix X s ss Htr); intro Hftr.
+  intros [| n].
+  - constructor. assumption.
+  - rewrite finite_trace_projection_stream.
+    apply finite_ptrace_projection; try assumption.
+    apply Hftr.
+Qed.
+
+(* The projection of an protocol trace remains a protocol trace *)
+
+Lemma ptrace_from_projection
+  (Hproj_dec : in_projection_dec)
+  (tr : vTrace X)
+  (Psj : protocol_state_prop Xj (trace_first tr j))
+  (Htr : ptrace_from_prop X tr)
+   : ptrace_from_prop Xj (trace_projection Hproj_dec tr).
+Proof.
+  destruct tr as [s ls | s ss].
+  - apply finite_ptrace_projection; assumption.
+  - simpl. destruct (Hproj_dec ss) as [[n _]|Hinf].
+    + apply finite_ptrace_projection; try assumption.
+      apply infinite_protocol_trace_from_prefix. assumption.
+    + destruct Hinf as [ks HFilter].
+      apply infinite_ptrace_projection; assumption.
+Qed.
+
+Lemma protocol_trace_projection
+  (Hproj_dec : in_projection_dec)
+  (tr : vTrace X)
+  (Htr : protocol_trace_prop X tr)
+  : protocol_trace_prop Xj (trace_projection Hproj_dec tr).
+Proof.
+  assert (Hfrom := protocol_trace_from X tr Htr).
+  assert (Hinit := protocol_trace_initial X tr Htr).
+  apply protocol_trace_from_iff.
+  split.
+  - apply ptrace_from_projection; try assumption.
+    apply protocol_state_prop_iff.
+    left.
+    apply (initial_state_projection IM constraint j) in Hinit.
+    exists (exist _ _ Hinit).
+    reflexivity.
+  - rewrite trace_projection_initial_state.
+    apply initial_state_projection.
+    assumption.
+Qed.
+
+(* We axiomatize projection friendliness as the converse of protocol_trace_projection *)
+Definition finite_projection_friendly
+  := forall
+    (sj : vstate (IM j))
+    (trj : list (vtransition_item (IM j)))
+    (Htrj : finite_protocol_trace Xj sj trj),
+    exists (sx : vstate X) (trx : list (vtransition_item X)),
+      finite_protocol_trace X sx trx
+      /\ sx j = sj
+      /\ finite_trace_projection_list trx = trj.
+
+Definition projection_friendly
+  (Hproj_dec : in_projection_dec)
+  := forall
+  (trj : vTrace (IM j))
+  (Htrj : protocol_trace_prop Xj trj),
+  exists (tr : vTrace X),
+    protocol_trace_prop X tr
+    /\ trace_projection Hproj_dec tr = trj.
+
+Lemma projection_friendly_finite
+  (Hproj_dec : in_projection_dec)
+  (Hfr : projection_friendly Hproj_dec)
+  : finite_projection_friendly.
+Proof.
+  unfold finite_projection_friendly;  intros.
+  specialize (Hfr (Finite sj trj) Htrj).
+  destruct Hfr as [[s tr| s tr] [Htr Heq]].
+  + exists s. exists tr.
+    split; try assumption.
+    unfold trace_projection in Heq.
+    inversion Heq.
+    split; reflexivity.
+  + unfold trace_projection in Heq.
+    destruct (Hproj_dec tr) as [[n1 _] | (ks, Hfilter)]; inversion Heq.
+    subst; clear Heq.
+    exists s. exists (stream_prefix tr n1).
+    destruct Htr as [Htr Hinit].
+    repeat split; try reflexivity; try assumption.
+    apply infinite_protocol_trace_from_prefix.
+    assumption.
+Qed.
+
+Lemma projection_friendly_in_futures'
+  (sx: state)
+  (trx: list transition_item)
+  (Htrx: finite_protocol_trace X sx trx)
+  (sj: state)
+  (Hsx: sx j = sj)
+  (Hall: Forall from_projection
+         (filter (fun a => bool_decide (from_projection a)) trx))
+  (s1 s2: state)
+  (n1 n2: nat)
+  (Hle: n1 <= n2)
+  (Hs1: nth_error
+        (sj
+         :: List.map destination (finite_trace_projection_list_alt trx Hall))
+        n1 = Some s1)
+  (Hs2: nth_error
+        (sj
+         :: List.map destination (finite_trace_projection_list_alt trx Hall))
+        n2 = Some s2)
+  : exists sX1 sX2 : vstate X, sX1 j = s1 /\ sX2 j = s2 /\ in_futures X sX1 sX2.
+Proof.
+    assert
+      (HsX1 :
+        exists (nX1 nX2 : nat) (sX1 sX2 : vstate X),
+          nX1 <= nX2 /\ sX1 j = s1 /\ sX2 j = s2
+          /\ nth_error (sx :: List.map destination trx) nX1 = Some sX1
+          /\ nth_error (sx :: List.map destination trx) nX2 = Some sX2
+      ).
+    {
+      destruct n1; destruct n2.
+      - exists 0; exists 0; exists sx; exists sx
+        ; inversion Hs1; inversion Hs2; subst; repeat split; assumption.
+      - exists 0; inversion Hs1; clear Hs1; subst.
+        simpl in Hs2.
+        rewrite nth_error_map in Hs2.
+        unfold finite_trace_projection_list_alt in Hs2.
+        rewrite nth_error_map in Hs2.
+        specialize
+          (nth_error_list_annotate
+            from_projection
+            (filter (fun a => bool_decide (from_projection a)) trx)
+            Hall
+            n2
+          ); intros [oitem [Hoa Hnth]].
+        match type of Hs2 with
+        | option_map _ (option_map _ ?n) = _ => replace n with oitem in Hs2
+        end.
+        clear Hoa.
+        destruct oitem as [[item Hitem]|]; try inversion Hs2; subst; clear Hs2.
+        simpl in Hnth.
+        symmetry in Hnth.
+        apply nth_error_filter in Hnth.
+        destruct Hnth as [nX2 [Hindex Hnth]].
+        exists (S nX2).
+        exists sx.
+        exists (destination item).
+        repeat split.
+        + lia.
+        + simpl. rewrite nth_error_map.
+          replace
+            (@nth_error (@transition_item message (@composite_type message index IM)) trx nX2)
+            with (Some item).
+          reflexivity.
+      - inversion Hle.
+      - simpl in Hs1. simpl in Hs2.
+        rewrite nth_error_map in Hs1.
+        rewrite nth_error_map in Hs2.
+        unfold finite_trace_projection_list_alt in Hs1.
+        unfold finite_trace_projection_list_alt in Hs2.
+        rewrite nth_error_map in Hs1.
+        rewrite nth_error_map in Hs2.
+        specialize
+          (nth_error_list_annotate
+            from_projection
+            (filter (fun a => bool_decide (from_projection a)) trx)
+            Hall
+            n2
+          ); intros [oitem2 [Hoa2 Hn2th]].
+        specialize
+          (nth_error_list_annotate
+            from_projection
+            (filter (fun a => bool_decide (from_projection a)) trx)
+            Hall
+            n1
+          ); intros [oitem1 [Hoa1 Hn1th]].
+        match type of Hs2 with
+        | option_map _ (option_map _ ?n) = _ => replace n with oitem2 in Hs2
+        end.
+        match type of Hs1 with
+        | option_map _ (option_map _ ?n) = _ => replace n with oitem1 in Hs1
+        end.
+        clear Hoa1.
+        destruct oitem2 as [[item2 Hitem2]|]; try inversion Hs2; subst; clear Hs2.
+        destruct oitem1 as [[item1 Hitem1]|]; try inversion Hs1; subst; clear Hs1.
+        simpl in Hn1th.
+        simpl in Hn2th.
+        symmetry in Hn1th.
+        symmetry in Hn2th.
+        apply nth_error_filter in Hn1th.
+        apply nth_error_filter in Hn2th.
+        destruct Hn2th as [nX2 [Hindex2 Hn2th]].
+        destruct Hn1th as [nX1 [Hindex1 Hn1th]].
+        exists (S nX1).
+        exists (S nX2).
+        exists (destination item1).
+        exists (destination item2).
+        repeat split; try assumption.
+        + assert (Hle' : n1 <= n2) by lia.
+          specialize (nth_error_filter_index_le _ _ _ _ Hle' _ _ Hindex1 Hindex2).
+          intro; lia.
+        + simpl. rewrite nth_error_map.
+          replace (@nth_error (@transition_item message (@composite_type message index IM)) trx nX1)
+            with (Some item1).
+          reflexivity.
+        + simpl. rewrite nth_error_map.
+          replace (@nth_error (@transition_item message (@composite_type message index IM)) trx nX2)
+            with (Some item2).
+          reflexivity.
+    }
+    destruct HsX1 as [nX1 [nX2 [sX1 [sX2 [HleX [Hps1 [Hps2 [HsX1 HsX2]]]]]]]].
+    exists sX1. exists sX2. repeat split; try assumption.
+    specialize (in_futures_witness_reverse X sX1 sX2 (exist (protocol_trace_prop X) (Finite sx trx) Htrx) nX1 nX2 HleX HsX1 HsX2).
+    intros; assumption.
+Qed.
+
+Lemma projection_friendly_in_futures
+  (Hfr : finite_projection_friendly)
+  (s1 s2 : vstate (IM j))
+  (Hfuture : in_futures Xj s1 s2)
+  : exists (sX1 sX2 : vstate X),
+    sX1 j = s1 /\ sX2 j = s2 /\ in_futures X sX1 sX2.
+Proof.
+  specialize (in_futures_witness Xj s1 s2 Hfuture)
+  ; intros [trj [n1 [n2 [Hle [Hs1 Hs2]]]]].
+  clear Hfuture.
+  destruct trj as [trj Htrj].
+  specialize (trace_prefix_fn_protocol Xj trj Htrj n2); intros Hpref.
+  remember (trace_prefix_fn Xj trj n2) as trj2.
+  destruct trj2 as [sj' lj' | sj' lj']; destruct trj as [sj lj | sj lj]
+  ; inversion Heqtrj2
+  ; subst sj' lj'.
+  - specialize (Hfr sj (list_prefix lj n2) Hpref).
+    destruct Hfr as [sx [trx [Htrx [Hsx Hproj]]]].
+    assert (Hall : Forall from_projection
+              (filter (fun a => bool_decide (from_projection a)) trx))
+      by apply filter_Forall.
+    specialize (finite_trace_projection_list_alt_iff trx Hall); intro Heq.
+    rewrite <- Heq in Hproj.
+    simpl in Hs1.
+    simpl in Hs2.
+    assert
+      (Hs1' :
+        nth_error (sj :: List.map destination lj) n1 =
+        nth_error (sj :: List.map destination (list_prefix lj n2)) n1
+      ).
+    { destruct n1; try reflexivity. simpl.
+      rewrite list_prefix_map.
+      symmetry. apply list_prefix_nth. assumption.
+    }
+    assert
+      (Hs2' :
+        nth_error (sj :: List.map destination lj) n2 =
+        nth_error (sj :: List.map destination (list_prefix lj n2)) n2
+      ).
+    { destruct n2; try reflexivity. simpl.
+      rewrite list_prefix_map.
+      symmetry. apply list_prefix_nth. constructor.
+    }
+    apply projection_friendly_in_futures' with sx trx sj Hall n1 n2; try assumption
+    ; rewrite Hproj.
+    + rewrite <- Hs1. symmetry. assumption.
+    + rewrite <- Hs2. symmetry. assumption.
+  - specialize (Hfr sj (stream_prefix lj n2) Hpref).
+    destruct Hfr as [sx [trx [Htrx [Hsx Hproj]]]].
+    assert (Hall : Forall from_projection
+              (filter (fun a => bool_decide (from_projection a)) trx))
+      by apply filter_Forall.
+    specialize (finite_trace_projection_list_alt_iff trx Hall); intro Heq.
+    rewrite <- Heq in Hproj.
+    simpl in Hs1.
+    simpl in Hs2.
+    assert
+      (Hs1' :
+        Some (Str_nth n1 (Cons sj (map destination lj))) =
+        nth_error (sj :: List.map destination (stream_prefix lj n2)) n1
+      ).
+    { destruct n1; try reflexivity. simpl.
+      rewrite stream_prefix_map.
+      rewrite stream_prefix_nth; try assumption.
+      reflexivity.
+    }
+    assert
+      (Hs2' :
+      Some (Str_nth n2 (Cons sj (map destination lj))) =
+        nth_error (sj :: List.map destination (stream_prefix lj n2)) n2
+      ).
+    { destruct n2; try reflexivity.
+      rewrite stream_prefix_map.
+      remember (S n2) as sn2. rewrite Heqsn2 at 3.
+      simpl.
+      rewrite stream_prefix_nth; subst; constructor.
+    }
+    apply projection_friendly_in_futures' with sx trx sj Hall n1 n2; try assumption
+    ; rewrite Hproj; rewrite <- Hs1 || rewrite <- Hs2; symmetry; assumption.
+Qed.
+
+End ProjectionTraces.
+
+Section ProjectionTraces_membership.
+
+Context
+  {message : Type}
+  {index : Type}
+  {IndEqDec : EqDecision index}
+  (IM : index -> VLSM message)
+  {i0 : Inhabited index}
+  (constraint : composite_label IM -> composite_state IM * option message -> Prop)
+  (X := composite_vlsm IM constraint)
+  .
+
+Lemma finite_trace_projection_list_in
+  (tr : list (vtransition_item X))
+  (itemX : vtransition_item X)
+  (HitemX : In itemX tr)
+  (j := projT1 (l itemX))
+  : In (@Build_transition_item _ (type (IM j)) (projT2 (l itemX)) (input itemX) (destination itemX j) (output itemX)) (finite_trace_projection_list IM j tr).
+Proof.
+  induction tr; [inversion HitemX|].
+  destruct HitemX as [HitemX | HitemX].
+  - simpl. subst a. unfold j in *. clear j.
+    match goal with
+    |- context [decide ?eq] => destruct (decide eq)
+    end
+    ; [| elim n; reflexivity].
+    left.
+    f_equal.
+    replace e with (@eq_refl index (projT1 (l itemX))) by apply UIP.
+    reflexivity.
+  - spec IHtr HitemX.
+    simpl.
+    match goal with
+    |- context [decide ?eq] => destruct (decide eq)
+    end
+    ;[|assumption].
+    right. assumption.
+Qed.
+
+Lemma finite_trace_projection_list_in_rev
+  (tr : list (composite_transition_item IM))
+  (j : index)
+  (itemj : vtransition_item (IM j))
+  (Hitemj : In itemj  (finite_trace_projection_list IM j tr))
+  : exists
+    (itemX : composite_transition_item IM)
+    (Houtput : output itemX = output itemj)
+    (Hinput : input itemX = input itemj)
+    (Hl1 : j = projT1 (l itemX))
+    (Hl2 : eq_rect_r _ (projT2 (l itemX)) Hl1 = l itemj)
+    (Hdestination : destination itemX j = destination itemj),
+    In itemX tr.
+Proof.
+  induction tr; [contradict Hitemj|].
+  simpl in Hitemj.
+  match type of Hitemj with
+  | context [decide ?eq] => destruct (decide eq)
+  end.
+  - destruct Hitemj as [Hitemj | Hitemj].
+    + subst itemj. simpl. exists a. exists eq_refl. exists eq_refl. exists e.
+      exists eq_refl. exists eq_refl. left. reflexivity.
+    + spec IHtr Hitemj.
+      destruct IHtr as [itemX [Houtput [Hinput [Hl1 [Hl2 [Hdestination HitemX]]]]]].
+      exists itemX. repeat split; [assumption| assumption |].
+      exists Hl1. exists Hl2. exists Hdestination. right. assumption.
+  - spec IHtr Hitemj.
+    destruct IHtr as [itemX [Houtput [Hinput [Hl1 [Hl2 [Hdestination HitemX]]]]]].
+    exists itemX. repeat split; [assumption| assumption |].
+    exists Hl1. exists Hl2. exists Hdestination. right. assumption.
+Qed.
+
+End ProjectionTraces_membership.
